Refactor

interfaces/ua_congruence.v
@@ -1,5 +1,9 @@
 Require Import
   Coq.Unicode.Utf8
+  HoTT.Basics.Equivalences
+  HoTT.Types.Forall
+  HoTT.Types.Sigma
+  HoTT.Types.Record
   HoTTClasses.interfaces.ua_algebra
   HoTT.Classes.interfaces.abstract_algebra
   HoTT.Basics.Overture.
@@ -7,31 +11,64 @@ Require Import
 Import algebra_notations.
 
 (* TODO. Fix doc. *)
-
-(** This section develops the [quotient_algebra] instance of the [Algebra] type
-    class. *)
-
-Section congruence.
+Section congruence_property.
   Context {σ : Signature} (A : Algebra σ) (Φ : ∀ s, relation (A s)).
 
-  (** The relation family [Φ] satisfies the [CongruenceProperty f] with respect
-      to the algebra operation [f : A s1 → A s2 → ... → A (s(n+1))] if
+(** The relation family [Φ] satisfies the [CongruenceProperty f] with respect
+    to the algebra operation [f : A s1 → A s2 → ... → A (s(n+1))] if
 
-        [Φ s1 x1 y1 ∧ Φ s2 x2 y2 ∧ ... ∧ Φ sn xn yn] implies
-        [Φ (s(n+1)) (f x1 x2 ... xn) (f y1 y2 ... yn)]. *)
+      [Φ s1 x1 y1 ∧ Φ s2 x2 y2 ∧ ... ∧ Φ sn xn yn] implies
+      [Φ (s(n+1)) (f x1 x2 ... xn) (f y1 y2 ... yn)]. *)
 
-  Definition CongruenceProperty {w : SymbolType σ} (f : Operation A w) : Type
+  Definition CongruenceProperty {w : SymbolType σ} (f : Operation A w)
+    : Type
     := ∀ (a b : FamilyProd A (dom_symboltype w)),
        for_all_2_family_prod A A Φ a b ->
        Φ (cod_symboltype w) (ap_operation f a) (ap_operation f b).
+
+  Class HasCongruenceProperty : Type
+    := has_congruence_property : ∀ (u : Symbol σ), CongruenceProperty (u^^A).
+End congruence_property.
+
+Arguments has_congruence_property {σ} A Φ {HasCongruenceProperty}.
+
+Section congruence.
+  Context {σ : Signature} (A : Algebra σ).
 
   (** The relation family [Φ] is a [IsCongruence] if [Φ s] it is a family of
       mere equivalence relations and [Φ] has the [CongruenceProperty f]
       for all the algebra operations [f]. *)
 
-  Class IsCongruence {M : ∀ s, is_mere_relation (A s) (Φ s)}
-      {E : ∀ s, Equivalence (Φ s)} : Type
-      := congruence_properties : ∀ (u : Symbol σ), CongruenceProperty (u^^A).
+  Record Congruence : Type := BuildCongruence
+    { relation_congruence : ∀ (s : Sort σ), relation (A s)
+    ; is_mere_relation_congruence
+        : ∀ (s : Sort σ), is_mere_relation (A s) (relation_congruence s)
+    ; equivalence_congruence
+        : ∀ (s : Sort σ), Equivalence (relation_congruence s)
+    ; congruence_property : HasCongruenceProperty A relation_congruence }.
+
+  Global Existing Instance is_mere_relation_congruence.
+
+  Global Existing Instance equivalence_congruence.
+
+  Global Existing Instance congruence_property.
+
+  Global Coercion relation_congruence : Congruence >-> Funclass.
+
+  Definition SigCongruence : Type :=
+    { relation_congruence : ∀ (s : Sort σ), relation (A s)
+    | { _ : ∀ (s : Sort σ), is_mere_relation (A s) (relation_congruence s)
+      | { _ : ∀ (s : Sort σ), Equivalence (relation_congruence s)
+        | HasCongruenceProperty A relation_congruence }}}.
+
+  Lemma issig_congruence : Congruence <~> SigCongruence.
+  Proof.
+    apply symmetric_equiv.
+    unfold SigCongruence.
+    issig BuildCongruence relation_congruence is_mere_relation_congruence
+            equivalence_congruence congruence_property.
+  Defined.
 End congruence.
 
-Arguments congruence_properties {σ} A Φ {M} {E} {IsCongruence}.
+Arguments BuildCongruence {σ} {A} relation_congruence
+  {is_mere_relation_congruence} {equivalence_congruence} {congruence_property}.
